***NO_CI*** some more cleanup

examples/seplogic/SL.ExamplesAuto.fst
@@ -334,11 +334,13 @@ let sl_auto () : Tac unit =
 unfold let frame_wp (#a:Type) (wp:st_wp a) =
   fun post m -> frame_wp wp (frame_post post) m
 
+effect ST (a:Type) (wp:st_wp a) = STATE a (frame_wp wp)
+
 let swap_wp (r1 r2:ref int) =
   fun p m -> exists x y. m == ((r1 |> x) <*> (r2 |> y)) /\ (defined m /\ p () ((r1 |> y) <*> (r2 |> x)))
 
 let swap (r1 r2:ref int)
-     : STATE unit (frame_wp (swap_wp r1 r2)) by sl_auto
+     : ST unit (swap_wp r1 r2) by sl_auto
   = let x = !r1 in
     let y = !r2 in
     r1 := y;
@@ -348,14 +350,14 @@ let rotate_wp (r1 r2 r3:ref int) =
   fun p m -> exists x y z. m == ((r1 |> x) <*> ((r2 |> y) <*> (r3 |> z))) /\ (defined m /\ p () ((r1 |> z) <*> ((r2 |> x) <*> (r3 |> y))))
 
 let rotate (r1 r2 r3:ref int)
-  : STATE unit (frame_wp (rotate_wp r1 r2 r3)) by sl_auto
+  : ST unit (rotate_wp r1 r2 r3) by sl_auto
   = swap r2 r3;
     swap r1 r2
 
 let test (r1 r2:ref int) =
   (!r1)
 
-  <: STATE int (frame_wp (fun p m -> exists x y. m == ((r1 |> x) <*> (r2 |> y)) /\ (defined m /\ p x m)))
+  <: ST int (fun p m -> exists x y. m == ((r1 |> x) <*> (r2 |> y)) /\ (defined m /\ p x m))
 
   by sl_auto
 
@@ -365,11 +367,11 @@ let test (r1 r2:ref int) =
 let write_read (r1 r2:ref int) =
   (r1 := 2;
    !r2)
-  <: STATE int (frame_wp (fun p m -> exists x y. m == ((r1 |> x) <*> (r2 |> y)) /\ (defined m /\ p y ((r1 |> 2) <*> (r2 |> y)))))
+  <: ST int (fun p m -> exists x y. m == ((r1 |> x) <*> (r2 |> y)) /\ (defined m /\ p y ((r1 |> 2) <*> (r2 |> y))))
   by sl_auto
 
 let read_write (r1 r2:ref int) =
   (let x = !r1 in
    r2 := x)
-  <: STATE unit (frame_wp (fun p m -> exists x y. m == ((r1 |> x) <*> (r2 |> y)) /\ (defined m /\ p () ((r1 |> x) <*> (r2 |> x)))))
+  <: ST unit (fun p m -> exists x y. m == ((r1 |> x) <*> (r2 |> y)) /\ (defined m /\ p () ((r1 |> x) <*> (r2 |> x))))
   by sl_auto
